Lean4Lean/Theory/Typing/NormalEq.lean
@@ -5,21 +5,23 @@ namespace Lean4Lean
 
 open VExpr
 
-variable (IsDefEq : List VExpr → VExpr → VExpr → Prop) (Γ₀ : List VExpr) in
+variable (IsDefEqU : List VExpr → VExpr → VExpr → Prop) (Γ₀ : List VExpr) in
 inductive IsDefEqCtx : List VExpr → List VExpr → Prop
   | zero : IsDefEqCtx Γ₀ Γ₀
-  | succ : IsDefEqCtx Γ₁ Γ₂ → IsDefEq Γ₁ A₁ A₂ → IsDefEqCtx (A₁ :: Γ₁) (A₂ :: Γ₂)
+  | succ : IsDefEqCtx Γ₁ Γ₂ → IsDefEqU Γ₁ A₁ A₂ → IsDefEqCtx (A₁ :: Γ₁) (A₂ :: Γ₂)
 
 section
 set_option hygiene false
-local notation:65 Γ " ⊢ " e " : " A:36 => HasType Γ e A
-local notation:65 Γ " ⊢ " e1 " ≡ " e2:36 => IsDefEq Γ e1 e2
+local notation:65 Γ " ⊢ " e " : " A:36 => IsDefEq Γ e e A
+local notation:65 Γ " ⊢ " e1 " ≡ " e2:36 " : " A:36 => IsDefEq Γ e1 e2 A
+local notation:65 Γ " ⊢ " e1 " ≡ " e2:36 => IsDefEqU Γ e1 e2
 structure Typing where
   env : VEnv
   -- henv : env.Ordered
   univs : Nat
-  IsDefEq : List VExpr → VExpr → VExpr → Prop
-  HasType : List VExpr → VExpr → VExpr → Prop
+  IsDefEq : List VExpr → VExpr → VExpr → VExpr → Prop
+  IsDefEqU : List VExpr → VExpr → VExpr → Prop
+  mkU : Γ ⊢ e1 ≡ e2 : A → Γ ⊢ e1 ≡ e2
   Pat : (p : Pattern) → p.RHS × p.Check → Prop
   refl : Γ ⊢ e : A → Γ ⊢ e ≡ e
   symm : Γ ⊢ e₁ ≡ e₂ → Γ ⊢ e₂ ≡ e₁
@@ -52,22 +54,22 @@ structure Typing where
     Γ ⊢ df.lhs.instL ls ≡ df.rhs.instL ls
   extra : env.defeqs df → (∀ l ∈ ls, l.WF uvars) → ls.length = df.uvars →
     Γ ⊢ df.lhs.instL ls : df.type.instL ls
-  isDefEq_weakN_iff (W : Ctx.LiftN n k Γ Γ') :
+  isDefEqU_weakN_iff (W : Ctx.LiftN n k Γ Γ') :
     Γ' ⊢ e1.liftN n k ≡ e2.liftN n k ↔ Γ ⊢ e1 ≡ e2
-  hasType_weakN_iff (W : Ctx.LiftN n k Γ Γ') : Γ' ⊢ e.liftN n k : A.liftN n k ↔ Γ ⊢ e : A
-  hasTypeU_weakN_inv (W : Ctx.LiftN n k Γ Γ') : Γ' ⊢ e.liftN n k : A → ∃ A', Γ ⊢ e : A'
-  isDefEq_instN (W : Ctx.InstN Γ₀ e₀ A₀ k Γ₁ Γ)
+  isDefEq_weakN_iff (W : Ctx.LiftN n k Γ Γ') : Γ' ⊢ e1.liftN n k ≡ e2.liftN n k : A.liftN n k ↔ Γ ⊢ e1 ≡ e2 : A
+  isDefEq_weakN_inv (W : Ctx.LiftN n k Γ Γ') : Γ' ⊢ e1.liftN n k ≡ e2.liftN n k : A → ∃ A', Γ ⊢ e1 ≡ e2 : A'
+  isDefEqU_instN (W : Ctx.InstN Γ₀ e₀ A₀ k Γ₁ Γ)
     (H : Γ₁ ⊢ e1 ≡ e2) (h₀ : Γ₀ ⊢ e₀ : A₀) : Γ ⊢ e1.inst e₀ k ≡ e2.inst e₀ k
-  hasType_instN (W : Ctx.InstN Γ₀ e₀ A₀ k Γ₁ Γ)
-    (H : Γ₁ ⊢ e1 : A) (h₀ : Γ₀ ⊢ e₀ : A₀) : Γ ⊢ e1.inst e₀ k : A.inst e₀ k
+  isDefEq_instN (W : Ctx.InstN Γ₀ e₀ A₀ k Γ₁ Γ)
+    (H : Γ₁ ⊢ e1 ≡ e2 : A) (h₀ : Γ₀ ⊢ e₀ : A₀) : Γ ⊢ e1.inst e₀ k ≡ e2.inst e₀ k : A.inst e₀ k
   isDefEq_instL (hls : ∀ l ∈ ls, l.WF U')
     (H : Γ ⊢ e1 ≡ e2) : Γ.map (VExpr.instL ls) ⊢ e1.instL ls ≡ e2.instL ls
   hasType_instL (hls : ∀ l ∈ ls, l.WF U')
     (H : Γ ⊢ e : A) : Γ.map (VExpr.instL ls) ⊢ e.instL ls : A.instL ls
   instL_congr : (∀ l ∈ ls, l.WF univs) → (∀ l ∈ ls', l.WF univs) → List.Forall₂ (· ≈ ·) ls ls' →
     Γ ⊢ e : A → Γ.map (VExpr.instL ls) ⊢ e.instL ls ≡ e.instL ls'
-  isDefEq_DFC : IsDefEqCtx IsDefEq Γ₀ Γ₁ Γ₂ → Γ₁ ⊢ e1 ≡ e2 → Γ₂ ⊢ e1 ≡ e2
-  hasType_DFC : IsDefEqCtx IsDefEq Γ₀ Γ₁ Γ₂ → Γ₁ ⊢ e : A → Γ₂ ⊢ e : A
+  isDefEqU_DFC : IsDefEqCtx IsDefEqU Γ₀ Γ₁ Γ₂ → Γ₁ ⊢ e1 ≡ e2 → Γ₂ ⊢ e1 ≡ e2
+  isDefEq_DFC : IsDefEqCtx IsDefEqU Γ₀ Γ₁ Γ₂ → Γ₁ ⊢ e1 ≡ e2 : A → Γ₂ ⊢ e1 ≡ e2 : A
   has_type : Γ ⊢ e₁ ≡ e₂ → ∃ A, Γ ⊢ e₁ : A
   is_type : Γ ⊢ e : A → ∃ u, Γ ⊢ A : .sort u
   bvar_inv : Γ ⊢ .bvar i : V → ∃ A, Lookup Γ i A
@@ -86,49 +88,50 @@ structure Typing where
   pat_uniq : Pat p₁ r → Pat p₂ r' → Subpattern p₃ p₁ → p₂.inter p₃ = some p₄ →
     p₁ = p₂ ∧ p₂ = p₃ ∧ r ≍ r'
   pat_wf : Pat p r → p.Matches e m1 m2 → Γ ⊢ e : A →
-    r.2.OK (IsDefEq Γ) m1 m2 → Γ ⊢ e ≡ r.1.apply m1 m2
+    r.2.OK (IsDefEqU Γ) m1 m2 → Γ ⊢ e ≡ r.1.apply m1 m2
   extra_pat : env.defeqs df → (∀ l ∈ ls, l.WF uvars) → ls.length = df.uvars →
-    ∃ p r m1 m2, Pat p r ∧ p.Matches (df.lhs.instL ls) m1 m2 ∧ r.2.OK (IsDefEq Γ) m1 m2 ∧
+    ∃ p r m1 m2, Pat p r ∧ p.Matches (df.lhs.instL ls) m1 m2 ∧ r.2.OK (IsDefEqU Γ) m1 m2 ∧
     df.rhs.instL ls = r.1.apply m1 m2
-  pat_onArgs : Pat p r → p.Matches e m1 m2 → Γ ⊢ e : A → r.2.OK (IsDefEq Γ) m1 m2 →
+  pat_onArgs : Pat p r → p.Matches e m1 m2 → Γ ⊢ e : A → r.2.OK (IsDefEqU Γ) m1 m2 →
     p.OnArgs fun a => (∀ A B, ¬Γ ⊢ a : .forallE A B) ∧ (∀ p, Γ ⊢ a : p → ¬Γ ⊢ p : .sort .zero)
 
+abbrev Typing.HasType (TY : Typing) (Γ : List VExpr) (e A : VExpr) := TY.IsDefEq Γ e e A
 variable {TY : Typing}
 
-theorem Typing.symm_ctx (H : IsDefEqCtx TY.IsDefEq Γ₀ Γ₁ Γ₂) : IsDefEqCtx TY.IsDefEq Γ₀ Γ₂ Γ₁ := by
+theorem Typing.symm_ctx (H : IsDefEqCtx TY.IsDefEqU Γ₀ Γ₁ Γ₂) : IsDefEqCtx TY.IsDefEqU Γ₀ Γ₂ Γ₁ := by
   induction H with
   | zero => exact .zero
-  | succ h1 h2 ih => exact .succ ih (TY.isDefEq_DFC h1 (TY.symm h2))
+  | succ h1 h2 ih => exact .succ ih (TY.isDefEqU_DFC h1 (TY.symm h2))
 
+theorem Typing.IsDefEqU.weakN (W : Ctx.LiftN n k Γ Γ') :
+    TY.IsDefEqU Γ e1 e2 → TY.IsDefEqU Γ' (e1.liftN n k) (e2.liftN n k) := (TY.isDefEqU_weakN_iff W).2
 theorem Typing.IsDefEq.weakN (W : Ctx.LiftN n k Γ Γ') :
-    TY.IsDefEq Γ e1 e2 → TY.IsDefEq Γ' (e1.liftN n k) (e2.liftN n k) := (TY.isDefEq_weakN_iff W).2
-theorem Typing.HasType.weakN (W : Ctx.LiftN n k Γ Γ') :
-    TY.HasType Γ e A → TY.HasType Γ' (e.liftN n k) (A.liftN n k) := (TY.hasType_weakN_iff W).2
+    TY.IsDefEq Γ e1 e2 A → TY.IsDefEq Γ' (e1.liftN n k) (e2.liftN n k) (A.liftN n k) := (TY.isDefEq_weakN_iff W).2
 
-theorem Typing.IsDefEq.instN : Ctx.InstN Γ₀ e₀ A₀ k Γ₁ Γ → TY.IsDefEq Γ₁ e1 e2 →
-    TY.HasType Γ₀ e₀ A₀ → TY.IsDefEq Γ (e1.inst e₀ k) (e2.inst e₀ k) := TY.isDefEq_instN
-theorem Typing.HasType.instN : Ctx.InstN Γ₀ e₀ A₀ k Γ₁ Γ → TY.HasType Γ₁ e A →
-    TY.HasType Γ₀ e₀ A₀ → TY.HasType Γ (e.inst e₀ k) (A.inst e₀ k) := TY.hasType_instN
+theorem Typing.IsDefEqU.instN : Ctx.InstN Γ₀ e₀ A₀ k Γ₁ Γ → TY.IsDefEqU Γ₁ e1 e2 →
+    TY.HasType Γ₀ e₀ A₀ → TY.IsDefEqU Γ (e1.inst e₀ k) (e2.inst e₀ k) := TY.isDefEqU_instN
+theorem Typing.IsDefEq.instN : Ctx.InstN Γ₀ e₀ A₀ k Γ₁ Γ → TY.IsDefEq Γ₁ e₁ e₂ A →
+    TY.HasType Γ₀ e₀ A₀ → TY.IsDefEq Γ (e₁.inst e₀ k) (e₂.inst e₀ k) (A.inst e₀ k) := TY.isDefEq_instN
 
 theorem Pattern.Check.OK.weakN (W : Ctx.LiftN n k Γ Γ') {p : Pattern}
-    (ck : p.Check) {m1 m2} (H : ck.OK (TY.IsDefEq Γ) m1 m2) :
-    ck.OK (TY.IsDefEq Γ') m1 fun x => (m2 x).liftN n k := by
+    (ck : p.Check) {m1 m2} (H : ck.OK (TY.IsDefEqU Γ) m1 m2) :
+    ck.OK (TY.IsDefEqU Γ') m1 fun x => (m2 x).liftN n k := by
   refine H.map fun a b h => ?_
   simp only [← Pattern.RHS.liftN_apply]
   exact h.weakN W
 
 theorem Pattern.Check.OK.instN (W : Ctx.InstN Γ₀ e₀ A₀ k Γ₁ Γ) (H₀ : TY.HasType Γ₀ e₀ A₀)
-    {p : Pattern} (ck : p.Check) {m1 m2} (H : ck.OK (TY.IsDefEq Γ₁) m1 m2) :
-    ck.OK (TY.IsDefEq Γ) m1 fun x => (m2 x).inst e₀ k := by
+    {p : Pattern} (ck : p.Check) {m1 m2} (H : ck.OK (TY.IsDefEqU Γ₁) m1 m2) :
+    ck.OK (TY.IsDefEqU Γ) m1 fun x => (m2 x).inst e₀ k := by
   refine H.map fun a b h => ?_
   simp only [← Pattern.RHS.instN_apply]
   exact h.instN W H₀
 
 open Pattern.RHS in
-theorem Typing.IsDefEq.apply_pat
-    (ih : ∀ a A, TY.HasType Γ (m2 a) A →  TY.IsDefEq Γ (m2 a) (m2' a))
+theorem Typing.IsDefEqU.apply_pat
+    (ih : ∀ a A, TY.HasType Γ (m2 a) A →  TY.IsDefEqU Γ (m2 a) (m2' a))
     (he : TY.HasType Γ (apply m1 m2 r) A) :
-     TY.IsDefEq Γ (apply m1 m2 r) (apply m1 m2' r) := by
+     TY.IsDefEqU Γ (apply m1 m2 r) (apply m1 m2' r) := by
   induction r generalizing A with simp [apply] at he ⊢
   | fixed path c _ => exact TY.refl he
   | app hf ha ih1 ih2 =>
@@ -153,7 +156,7 @@ section
 set_option hygiene false
 variable (TY : Typing)
 local notation:65 Γ " ⊢ " e " : " A:30 => TY.HasType Γ e A
-local notation:65 Γ " ⊢ " e1 " ≡ " e2:30 => TY.IsDefEq Γ e1 e2
+local notation:65 Γ " ⊢ " e1 " ≡ " e2:30 => TY.IsDefEqU Γ e1 e2
 local notation:65 Γ " ⊢ " e1 " ≡ₚ " e2:30 => NormalEq Γ e1 e2
 
 inductive NormalEq : List VExpr → VExpr → VExpr → Prop where
@@ -193,7 +196,7 @@ inductive NormalEq : List VExpr → VExpr → VExpr → Prop where
 
 end
 
-theorem NormalEq.defeq (H : NormalEq TY Γ e1 e2) : TY.IsDefEq Γ e1 e2 := by
+theorem NormalEq.defeq (H : NormalEq TY Γ e1 e2) : TY.IsDefEqU Γ e1 e2 := by
   induction H with
   | refl h => exact TY.refl h
   | sortDF h1 h2 h3 => exact TY.sortDF h1 h2 h3
@@ -307,42 +310,42 @@ theorem NormalEq.instN_r (W : Ctx.InstN Γ₀ e₀ A₀ k Γ₁ Γ) (H : Typing.
     exact .forallEDF hA (TY.refl hA) (ih1 W h1) (h2.instN W.succ h₀) (ih2 W.succ h2)
 
 variable {TY : Typing} in
-theorem NormalEq.defeqDFC (W : IsDefEqCtx TY.IsDefEq Γ₀ Γ₁ Γ₂)
+theorem NormalEq.defeqDFC (W : IsDefEqCtx TY.IsDefEqU Γ₀ Γ₁ Γ₂)
     (H : NormalEq TY Γ₁ e1 e2) : NormalEq TY Γ₂ e1 e2 := by
   induction H generalizing Γ₂ with
-  | refl h => refine .refl (TY.hasType_DFC W h)
+  | refl h => refine .refl (TY.isDefEq_DFC W h)
   | sortDF h1 h2 h3 => exact .sortDF h1 h2 h3
   | constDF h1 h2 h3 h4 h5 => exact .constDF h1 h2 h3 h4 h5
   | appDF h1 h2 h3 h4 _ _ ih1 ih2 =>
-    exact .appDF (TY.hasType_DFC W h1) (TY.hasType_DFC W h2)
-      (TY.hasType_DFC W h3) (TY.hasType_DFC W h4) (ih1 W) (ih2 W)
+    exact .appDF (TY.isDefEq_DFC W h1) (TY.isDefEq_DFC W h2)
+      (TY.isDefEq_DFC W h3) (TY.isDefEq_DFC W h4) (ih1 W) (ih2 W)
   | lamDF h1 h2 h3 _ ih1 =>
-    exact .lamDF (TY.hasType_DFC W h1) (TY.isDefEq_DFC W h2) (TY.isDefEq_DFC W h3)
+    exact .lamDF (TY.isDefEq_DFC W h1) (TY.isDefEqU_DFC W h2) (TY.isDefEqU_DFC W h3)
       (ih1 (W.succ (TY.refl h1)))
   | forallEDF h1 h2 _ h4 _ ih1 ih2 =>
-    exact .forallEDF (TY.hasType_DFC W h1) (TY.isDefEq_DFC W h2) (ih1 W)
-      (TY.hasType_DFC (W.succ (TY.refl h1)) h4) (ih2 (W.succ (TY.refl h1)))
+    exact .forallEDF (TY.isDefEq_DFC W h1) (TY.isDefEqU_DFC W h2) (ih1 W)
+      (TY.isDefEq_DFC (W.succ (TY.refl h1)) h4) (ih2 (W.succ (TY.refl h1)))
   | etaL h1 _ ih =>
     have ⟨_, _, h2, _⟩ := let ⟨_, h⟩ := TY.is_type h1; TY.forallE_inv h
-    refine .etaL (TY.hasType_DFC W h1) (ih (W.succ (TY.refl h2)))
+    refine .etaL (TY.isDefEq_DFC W h1) (ih (W.succ (TY.refl h2)))
   | etaR h1 _ ih =>
     have ⟨_, _, h2, _⟩ := let ⟨_, h⟩ := TY.is_type h1; TY.forallE_inv h
-    refine .etaR (TY.hasType_DFC W h1) (ih (W.succ (TY.refl h2)))
+    refine .etaR (TY.isDefEq_DFC W h1) (ih (W.succ (TY.refl h2)))
   | proofIrrel h1 h2 h3 =>
-    exact .proofIrrel (TY.hasType_DFC W h1)
-      (TY.hasType_DFC W h2) (TY.hasType_DFC W h3)
+    exact .proofIrrel (TY.isDefEq_DFC W h1)
+      (TY.isDefEq_DFC W h2) (TY.isDefEq_DFC W h3)
 
-theorem NormalEq.defeq_l (W : TY.IsDefEq Γ A A') (H : NormalEq TY (A::Γ) e1 e2) :
+theorem NormalEq.defeq_l (W : TY.IsDefEqU Γ A A') (H : NormalEq TY (A::Γ) e1 e2) :
     NormalEq TY (A'::Γ) e1 e2 := defeqDFC (.succ .zero W) H
 
-theorem NormalEq.weakN_inv_DFC (W : Ctx.LiftN n k Γ Γ₂) (W₂ : IsDefEqCtx TY.IsDefEq Γ₀ Γ₁ Γ₂)
+theorem NormalEq.weakN_inv_DFC (W : Ctx.LiftN n k Γ Γ₂) (W₂ : IsDefEqCtx TY.IsDefEqU Γ₀ Γ₁ Γ₂)
     (H : NormalEq TY Γ₁ (e1.liftN n k) (e2.liftN n k)) : NormalEq TY Γ e1 e2 := by
   generalize eq1 : e1.liftN n k = e1' at H
   generalize eq2 : e2.liftN n k = e2' at H
   induction H generalizing Γ Γ₂ e1 e2 k with
   | refl h =>
     cases eq2; cases liftN_inj.1 eq1
-    have ⟨_, h'⟩ := TY.hasTypeU_weakN_inv W (TY.hasType_DFC W₂ h)
+    have ⟨_, h'⟩ := TY.isDefEq_weakN_inv W (TY.isDefEq_DFC W₂ h)
     exact .refl h'
   | sortDF h1 h2 h3 =>
     cases e1 <;> cases eq1
@@ -355,75 +358,77 @@ theorem NormalEq.weakN_inv_DFC (W : Ctx.LiftN n k Γ Γ₂) (W₂ : IsDefEqCtx T
   | appDF h1 h2 h3 h4 _ _ ih1 ih2 =>
     cases e1 <;> cases eq1
     cases e2 <;> cases eq2
-    replace h1 := TY.hasType_DFC W₂ h1
-    replace h2 := TY.hasType_DFC W₂ h2
-    replace h3 := TY.hasType_DFC W₂ h3
-    replace h4 := TY.hasType_DFC W₂ h4
+    replace h1 := TY.isDefEq_DFC W₂ h1
+    replace h2 := TY.isDefEq_DFC W₂ h2
+    replace h3 := TY.isDefEq_DFC W₂ h3
+    replace h4 := TY.isDefEq_DFC W₂ h4
     have ⟨_, _, l1, l2⟩ :=
-      let ⟨_, h⟩ := TY.hasTypeU_weakN_inv W (TY.app h1 h3) (e := .app ..); TY.app_inv h
+      let ⟨_, h⟩ := TY.isDefEq_weakN_inv W (TY.app h1 h3) (e1 := .app ..) (e2 := .app ..)
+      TY.app_inv h
     have ⟨_, _, r1, r2⟩ :=
-      let ⟨_, h⟩ := TY.hasTypeU_weakN_inv W (TY.app h2 h4) (e := .app ..); TY.app_inv h
-    have := (TY.isDefEq_weakN_iff W).1
+      let ⟨_, h⟩ := TY.isDefEq_weakN_inv W (TY.app h2 h4)  (e1 := .app ..) (e2 := .app ..)
+      TY.app_inv h
+    have := (TY.isDefEqU_weakN_iff W).1
       (TY.trans (TY.uniq (l1.weakN W) h1) (TY.uniq h2 (r1.weakN W)))
     exact .appDF (TY.defeq_r this l1) r1
       (TY.defeq_r (TY.forallE_defInv this).1 l2) r2 (ih1 W W₂ rfl rfl) (ih2 W W₂ rfl rfl)
   | lamDF h1 h2 h3 _ ih1 =>
     cases e1 <;> cases eq1
     cases e2 <;> cases eq2
-    have := (TY.hasType_weakN_iff (A := .sort ..) W).1 <|
-      TY.hasType_DFC W₂ (TY.defeq_l (TY.symm h2) h1)
-    have h5 := (TY.isDefEq_weakN_iff W).1 <| TY.isDefEq_DFC W₂ (TY.trans h3 (TY.symm h2))
+    have := (TY.isDefEq_weakN_iff (A := .sort ..) W).1 <|
+      TY.isDefEq_DFC W₂ (TY.defeq_l (TY.symm h2) h1)
+    have h5 := (TY.isDefEqU_weakN_iff W).1 <| TY.isDefEqU_DFC W₂ (TY.trans h3 (TY.symm h2))
     exact .lamDF this (TY.refl this) h5 (ih1 W.succ (W₂.succ (TY.symm h2)) rfl rfl)
   | forallEDF h1 h2 _ h4 _ ih1 ih2 =>
     cases e1 <;> cases eq1
     cases e2 <;> cases eq2
-    replace h4 := (TY.hasType_weakN_iff (A := .sort ..) W.succ).1 <|
-      TY.hasType_DFC (W₂.succ (TY.symm h2)) h4
-    have := (TY.hasType_weakN_iff (A := .sort ..) W).1 <|
-      TY.hasType_DFC W₂ (TY.defeq_l (TY.symm h2) h1)
+    replace h4 := (TY.isDefEq_weakN_iff (A := .sort ..) W.succ).1 <|
+      TY.isDefEq_DFC (W₂.succ (TY.symm h2)) h4
+    have := (TY.isDefEq_weakN_iff (A := .sort ..) W).1 <|
+      TY.isDefEq_DFC W₂ (TY.defeq_l (TY.symm h2) h1)
     exact .forallEDF this (TY.refl this)
       (ih1 W W₂ rfl rfl) h4 (ih2 W.succ (W₂.succ (TY.symm h2)) rfl rfl)
   | etaL h1 _ ih =>
     cases e1 <;> cases eq1
     subst eq2
     have ⟨_, _, hA, hB⟩ := let ⟨_, h⟩ := TY.is_type h1; TY.forallE_inv h
-    have h1' := TY.hasType_DFC W₂ h1
-    have hA' := TY.hasType_DFC W₂ hA
-    have hB' := TY.hasType_DFC (W₂.succ (TY.refl hA)) hB
+    have h1' := TY.isDefEq_DFC W₂ h1
+    have hA' := TY.isDefEq_DFC W₂ hA
+    have hB' := TY.isDefEq_DFC (W₂.succ (TY.refl hA)) hB
     have := TY.app (h1'.weakN .one) (TY.bvar .zero)
     rw [instN_bvar0, ← lift, lift_liftN',
       ← show liftN n (.bvar 0) (k+1) = bvar 0 by simp [liftN],
       ← liftN] at this
-    have ⟨C, hC⟩ := TY.hasTypeU_weakN_inv W.succ this
-    have := (TY.hasType_weakN_iff (A := .forallE ..) W).1 <|
+    have ⟨C, hC⟩ := TY.isDefEq_weakN_inv W.succ this
+    have := (TY.isDefEq_weakN_iff (A := .forallE ..) W).1 <|
       TY.defeq_r (TY.forallEDF hA' (TY.refl hA') hB' (TY.uniq this (hC.weakN W.succ))) h1'
     refine .etaL this (ih W.succ (W₂.succ (TY.refl hA)) rfl (by simp [liftN, lift_liftN']))
   | etaR h1 _ ih =>
     subst eq1
     cases e2 <;> cases eq2
     have ⟨_, _, hA, hB⟩ := let ⟨_, h⟩ := TY.is_type h1; TY.forallE_inv h
-    have h1' := TY.hasType_DFC W₂ h1
-    have hA' := TY.hasType_DFC W₂ hA
-    have hB' := TY.hasType_DFC (W₂.succ (TY.refl hA)) hB
+    have h1' := TY.isDefEq_DFC W₂ h1
+    have hA' := TY.isDefEq_DFC W₂ hA
+    have hB' := TY.isDefEq_DFC (W₂.succ (TY.refl hA)) hB
     have := TY.app (h1'.weakN .one) (TY.bvar .zero)
     rw [instN_bvar0, ← lift, lift_liftN',
       ← show liftN n (.bvar 0) (k+1) = bvar 0 by simp [liftN],
       ← liftN] at this
-    have ⟨C, hC⟩ := TY.hasTypeU_weakN_inv W.succ this
-    have := (TY.hasType_weakN_iff (A := .forallE ..) W).1 <|
+    have ⟨C, hC⟩ := TY.isDefEq_weakN_inv W.succ this
+    have := (TY.isDefEq_weakN_iff (A := .forallE ..) W).1 <|
       TY.defeq_r (TY.forallEDF hA' (TY.refl hA') hB' (TY.uniq this (hC.weakN W.succ))) h1'
     refine .etaR this (ih W.succ (W₂.succ (TY.refl hA)) (by simp [liftN, lift_liftN']) rfl)
   | proofIrrel h1 h2 h3 =>
     subst eq1; subst eq2
-    have h1' := TY.hasType_DFC W₂ h1
-    have h2' := TY.hasType_DFC W₂ h2
-    have h3' := TY.hasType_DFC W₂ h3
-    have ⟨_, h⟩ := TY.hasTypeU_weakN_inv W h2'
+    have h1' := TY.isDefEq_DFC W₂ h1
+    have h2' := TY.isDefEq_DFC W₂ h2
+    have h3' := TY.isDefEq_DFC W₂ h3
+    have ⟨_, h⟩ := TY.isDefEq_weakN_inv W h2'
     have hw := TY.uniq h2' (h.weakN W)
     exact .proofIrrel
-      ((TY.hasType_weakN_iff (A := .sort ..) W).1 (TY.defeq_l hw h1'))
-      ((TY.hasType_weakN_iff W).1 (TY.defeq_r hw h2'))
-      ((TY.hasType_weakN_iff W).1 (TY.defeq_r hw h3'))
+      ((TY.isDefEq_weakN_iff (A := .sort ..) W).1 (TY.defeq_l hw h1'))
+      ((TY.isDefEq_weakN_iff W).1 (TY.defeq_r hw h2'))
+      ((TY.isDefEq_weakN_iff W).1 (TY.defeq_r hw h3'))
 
 theorem NormalEq.weakN_iff (W : Ctx.LiftN n k Γ Γ') :
     NormalEq TY Γ' (e1.liftN n k) (e2.liftN n k) ↔ NormalEq TY Γ e1 e2 :=
